hide the inv in mont_loop_inv

otbn_model/code/mont_loop_lemmas.dfy
@@ -8,32 +8,88 @@ module mont_loop_lemmas {
     import opened powers
     import opened congruences
 
+    predicate mont_loop_inv(
+        x_i: uint256,
+        u_i: uint256,
+        m_0': uint256,
+        p_1: uint512_view_t,
+        p_2: uint512_view_t,
+        y: seq<uint256>,
+        m: seq<uint256>,
+        initial_a: seq<uint256>,
+        a: seq<uint256>,
+        j: nat)
+    {
+        && |m| == |a| == |y| == |initial_a| == NUM_WORDS;
+        && (1 <= j <= NUM_WORDS)
+        && (x_i * to_nat(y[..j]) + u_i * to_nat(m[..j]) + to_nat(initial_a[..j]) 
+            == 
+        to_nat([0] + a[..j-1]) + p_2.uh * pow_B256(j) + p_1.uh * pow_B256(j))
+    }
+
+    lemma mont_loop_divisible_lemma1
+        (x_i: uint256,
+        u_i: uint256,
+        m_0': uint256,
+        p_1: uint512_view_t,
+        p_2: uint512_view_t,
+        y_0: uint256,
+        m_0: uint256,
+        a_0: uint256)
+
+        requires p_1.full == x_i * y_0 + a_0;
+        requires p_2.full == u_i * m_0 + p_1.lh;
+        requires cong_B256(m_0' * m_0, BASE_256 - 1);
+        requires cong_B256(u_i, (a_0 + y_0 * x_i) * m_0');
+        ensures p_2.lh == 0;
+    {
+        assume false; // TODO
+    }
+
     lemma mont_loop_inv_lemma1(
         x_i: uint256,
         u_i: uint256,
+        m_0': uint256,
         p_1: uint512_view_t,
         p_2: uint512_view_t,
+        y: seq<uint256>,
         m: seq<uint256>,
-        A: seq<uint256>, 
-        y: seq<uint256>)
+        a: seq<uint256>)
 
-        requires |m| == |A| == |y| >= 1;
-        requires p_1.full == x_i * y[0]  + A[0];
+        requires |m| == |a| == |y| == NUM_WORDS;
+        requires cong_B256(m_0' * m[0], BASE_256 - 1);
+        requires p_1.full == x_i * y[0] + a[0];
         requires p_2.full == u_i * m[0] + p_1.lh;
-        requires p_2.lh == 0;
+        requires cong_B256(m_0' * m[0], BASE_256 - 1);
+        requires cong_B256(u_i, (a[0] + y[0] * x_i) * m_0');
 
-        ensures x_i * to_nat(y[..1]) + u_i * to_nat(m[..1]) + to_nat(A[..1])
-                == 
-            p_2.uh * pow_B256(1) + p_1.uh * pow_B256(1);
+        ensures mont_loop_inv(x_i, u_i, m_0', p_1, p_2, y, m, a, a, 1)
         {
+            mont_loop_divisible_lemma1(x_i, u_i, m_0', p_1, p_2, y[0], m[0], a[0]);
+
             to_nat_lemma1(y[..1]);
             to_nat_lemma1(m[..1]);
-            to_nat_lemma1(A[..1]);
+            to_nat_lemma1(a[..1]);
 
             assert p_2.full == p_2.uh * BASE_256 by {
                 uint512_view_lemma(p_2);
             }
 
             uint512_view_lemma(p_1);
+
+            calc == {
+                x_i * to_nat(y[..1]) + u_i * to_nat(m[..1]) + to_nat(a[..1]);
+                p_2.uh * pow_B256(1) + p_1.uh * pow_B256(1);
+                {
+                    assert to_nat([0]) == 0 by {
+                        reveal to_nat();
+                    }
+                }
+                to_nat([0]) + p_2.uh * pow_B256(1) + p_1.uh * pow_B256(1);
+                {
+                    assert [0] + a[..0] == [0];
+                }
+                to_nat([0] + a[..0]) + p_2.uh * pow_B256(1) + p_1.uh * pow_B256(1);
+            }
         }
 }
